live, unused_in from references to locs

ulib/FStar.ModifiesGen.fst
@@ -1468,6 +1468,19 @@ let modifies_address_liveness_insensitive_unused_in #al c h h' =
 
 #reset-options
 
+let mreference_live_loc_not_unused_in #al c #t #pre h b =
+  Classical.move_requires (does_not_contain_addr_addr_unused_in h) (HS.frameOf b, HS.as_addr b);
+  assert (~ (h `does_not_contain_addr` (HS.frameOf b, HS.as_addr b)));
+  loc_addresses_not_unused_in c (HS.frameOf b) (Set.singleton (HS.as_addr b)) h;
+  loc_includes_trans (loc_not_unused_in c h) (loc_freed_mreference b) (loc_mreference b);
+  ()
+
+let mreference_unused_in_loc_unused_in #al c #t #pre h b =
+  Classical.move_requires (addr_unused_in_does_not_contain_addr h) (HS.frameOf b, HS.as_addr b);
+  loc_addresses_unused_in c (HS.frameOf b) (Set.singleton (HS.as_addr b)) h;
+  loc_includes_addresses_addresses c false true (HS.frameOf b) (Set.singleton (HS.as_addr b)) (Set.singleton (HS.as_addr b));
+  loc_includes_trans (loc_unused_in c h) (loc_freed_mreference b) (loc_mreference b);
+  ()
 
 (* * Compositionality *)
 
